progress on parser soundness proof

coq/Parser_sound.v
@@ -1,7 +1,8 @@
-Require Import Arith List Logic.JMeq.
+Require Import Arith List.
 Require Import GallStar.Defs. 
 Require Import GallStar.Lex.
 Require Import GallStar.Parser.
+Require Import GallStar.Prediction.
 Require Import GallStar.Tactics.
 Require Import GallStar.Termination.
 
@@ -17,6 +18,22 @@ Program Fixpoint bottomFrame (stk : p_stack) {measure (stackSize stk)} : frame :
   | (fr, [])       => fr
   | (_, fr :: frs) => bottomFrame (fr, frs)
   end.
+
+Inductive bottom_frame : frame -> p_stack -> Prop :=
+| BF_nil :
+    forall fr,
+      bottom_frame fr (fr, [])
+| BF_cons :
+    forall b_fr fr1 fr2 frs,
+    bottom_frame b_fr (fr2, frs)
+    -> bottom_frame b_fr (fr1, fr2 :: frs).
+
+Lemma test :
+  forall stk a b c,
+    stk = (a, [b; c]) -> bottom_frame c stk.
+Proof.
+  intros stk a b c heq; subst; repeat constructor.
+Qed.
 
 Lemma bottomFrame_rew :
   forall (stk : p_stack),
@@ -63,12 +80,11 @@ Lemma multistep_unfold :
   forall g st a,
     multistep g st a = 
     match step g st as res return (step g st = res -> parse_result) with
-    | StepAccept sv => fun _ : step g st = StepAccept sv => Accept sv
-    | StepReject s => fun _ : step g st = StepReject s => Reject s
-    | StepK st' =>
-      fun Hs : step g st = StepK st' =>
-        multistep g st' (StepK_st_acc g st st' a Hs)
-    | StepError s => fun _ : step g st = StepError s => Error s
+    | StepAccept sv => fun _  => Accept sv
+    | StepReject s  => fun _  => Reject s
+    | StepK st'     => fun hs =>
+                         multistep g st' (StepK_st_acc g st st' a hs)
+    | StepError s   => fun _  => Error s
     end eq_refl.
 Proof.
   intros; destruct a; auto.
@@ -77,7 +93,7 @@ Qed.
 Lemma multistep_cases' :
   forall (g   : grammar)
          (st  : parser_state)
-         (a   : Acc lex_nat_triple (meas g st))
+         (a   : Acc lex_nat_triple (Parser.meas g st))
          (sr  : step_result)
          (pr  : parse_result)
          (heq : step g st = sr),
@@ -100,19 +116,14 @@ Lemma multistep_cases' :
        end.
 Proof.
   intros g st a sr pr heq.
-  destruct pr; destruct sr; subst; try solve [intros; congruence].
-  - intros h; inv h; auto.
-  - intros h; right; eauto.
-  - intros h; inv h; auto.
-  - intros h; right; eauto.
-  - intros h; right; eauto.
-  - intros h; inv h; auto.
+  destruct pr; destruct sr; subst;
+    try solve [ intros; tc | intros h; inv h; auto | intros h; right; eauto ].
 Qed.
 
 Lemma multistep_cases :
   forall (g : grammar)
          (st : parser_state)
-         (a  : Acc lex_nat_triple (meas g st))
+         (a  : Acc lex_nat_triple (Parser.meas g st))
          (pr  : parse_result),
     multistep g st a = pr
     -> match pr with
@@ -132,10 +143,10 @@ Proof.
   eapply multistep_cases'; eauto.
 Qed.
 
-Lemma multistep_accept :
+Lemma multistep_accept_cases :
   forall (g : grammar)
          (st : parser_state)
-         (a  : Acc lex_nat_triple (meas g st))
+         (a  : Acc lex_nat_triple (Parser.meas g st))
          (f  : forest),
     multistep g st a = Accept f
     -> step g st = StepAccept f
@@ -146,49 +157,308 @@ Proof.
   destruct (multistep_cases g st a (Accept f)); auto.
 Qed.
 
+Definition frame_derivation_invar g fr : Prop :=
+  exists wpre, gamma_derivation g fr.(loc).(rpre) wpre fr.(sem).
+
+Lemma step_StepAccept_facts :
+  forall g av stk ts v,
+    step g (Pst av stk ts) = StepAccept v
+    -> (exists xo rpre v',
+           stk = (Fr (Loc xo rpre []) v', [])
+           /\ v' = v)
+       /\ ts = [].
+Proof.
+  intros g av stk ts v hs.
+  unfold step in hs; dms; tc.
+  inv hs; repeat eexists; eauto.
+Qed.
+
+
+(* I should be able to get the wsuf out of this definition *)
+Inductive stack_derives_prefix (g : grammar) : p_stack -> list token -> list token -> Prop :=
+| Nil_sdp :
+    forall xo gpre gsuf wpre wsuf v,
+    gamma_derivation g gpre wpre v
+    -> stack_derives_prefix g (Fr (Loc xo gpre gsuf) v, []) wpre wsuf
+| Cons_sdp :
+    forall xo gpre gsuf wpre wpre' wsuf v fr frs,
+    gamma_derivation g gpre wpre' v
+    -> stack_derives_prefix g (fr, frs) wpre (wpre' ++ wsuf)
+    -> stack_derives_prefix g (Fr (Loc xo gpre gsuf) v, fr :: frs) (wpre ++ wpre') wsuf.
+
+Inductive stack_wf (g : grammar) : p_stack -> Prop :=
+| Nil_wf :
+    forall pre suf v,
+      stack_wf g (Fr (Loc None pre suf) v, [])
+| Cons_wf :
+    forall x xo pre pre' suf suf' v v' frs,
+      In (x, pre' ++ suf') g
+      -> stack_wf g (Fr (Loc (Some x) pre' suf') v',
+                     (Fr (Loc xo pre (NT x :: suf)) v) :: frs).
+
+Lemma stack_invariant_accept_implies_bottom_frame_rpre_derives_result :
+  forall fr stk g wpre wsuf av ts v,
+  bottom_frame fr stk
+  -> stack_derives_prefix g stk wpre wsuf
+  -> step g (Pst av stk ts) = StepAccept v
+  -> gamma_derivation g fr.(loc).(rpre) wpre v.
+Proof.
+  intros fr stk g wpre wsuf av ts v hb hsdp hf.
+  apply step_StepAccept_facts in hf.
+  destruct hf as [[xo [rpre [v' [heq heq']]]] hnil].
+  subst.
+  inv hb.
+  inv hsdp.
+  simpl; auto.
+Qed.
+
+Lemma bar :
+  forall g ys1 w1 v1,
+    gamma_derivation g ys1 w1 v1
+    -> forall ys2 w2 v2,
+      gamma_derivation g ys2 w2 v2
+      -> gamma_derivation g (ys1 ++ ys2) (w1 ++ w2) (v1 ++ v2).
+Proof.
+  intros g ys1 w1 v1 hg.
+  induction hg; intros ys2 w2 v2 hg2; simpl in *; auto.
+  rewrite <- app_assoc.
+  constructor; auto.
+Qed.
+
+Lemma app_nil_r' : forall A (xs : list A), xs = xs ++ [].
+Proof.
+  intros; rewrite app_nil_r; auto.
+Qed.
+
+Lemma foo :
+  forall g xo rpre rpre2 x rsuf v1 v2 frs w1 w2 w3,
+    stack_derives_prefix g (Fr (Loc xo rpre (NT x :: rsuf)) v1, frs) w1 (w2 ++ w3)
+    -> In (x, rpre2) g
+    -> gamma_derivation g rpre2 w2 v2
+    -> stack_derives_prefix g (Fr (Loc xo (rpre ++ [NT x]) rsuf) (v1 ++ [Node x v2]), frs) (w1 ++ w2) w3.
+Proof.
+  intros g xo rpre rpre2 x rsuf v1 v2 frs w1 w2 w3 hi hin hg.
+  inv hi.
+  - constructor.
+    apply bar; auto.
+    assert (happ : w2 = w2 ++ []) by (apply app_nil_r'); rewrite happ.
+    repeat econstructor; eauto.
+  - rewrite <- app_assoc; constructor.
+    + apply bar; auto.
+      assert (happ : w2 = w2 ++ []) by (apply app_nil_r').
+      rewrite happ; repeat econstructor; eauto.
+    + rewrite <- app_assoc; auto.
+Qed.
+
+Lemma foo' :
+  forall g xo pre a suf v frs wpre l wsuf',
+    stack_derives_prefix g
+                         (Fr (Loc xo pre (T a :: suf)) v, frs)
+                         wpre
+                         ((a, l) :: wsuf')
+    -> stack_derives_prefix g
+                            (Fr (Loc xo (pre ++ [T a]) suf) (v ++ [Leaf l]), frs)
+                            (wpre ++ [(a, l)])
+                            wsuf'.
+Proof.
+  intros g xo pre a suf v frs wpre l wsuf' hinv.
+  inv hinv.
+  - constructor.
+    apply bar; auto.
+    (* lemma *)
+    assert (happ : [(a, l)] = [(a, l)] ++ []) by (apply app_nil_r'); rewrite happ; clear happ.
+        assert (happ : [Leaf l] = [Leaf l] ++ []) by (apply app_nil_r'); rewrite happ; clear happ.
+        econstructor; eauto.
+        constructor.
+        constructor.
+  - rewrite <- app_assoc.
+    constructor.
+    + apply bar; auto.
+      assert (happ : [(a, l)] = [(a, l)] ++ []) by (apply app_nil_r'); rewrite happ; clear happ.
+      assert (happ : [Leaf l] = [Leaf l] ++ []) by (apply app_nil_r'); rewrite happ; clear happ.
+      econstructor; eauto.
+      constructor.
+      constructor.
+    + rewrite <- app_assoc; auto.
+Qed.
+
+Lemma step_preserves_inv :
+  forall g av av' stk stk' wpre wsuf wsuf',
+    stack_wf g stk
+    -> stack_derives_prefix g stk wpre wsuf
+    -> step g (Pst av stk wsuf) = StepK (Pst av' stk' wsuf')
+    -> exists wpre',
+      wpre ++ wsuf = wpre' ++ wsuf'
+      /\ stack_derives_prefix g stk' wpre' wsuf'.
+Proof.
+  intros g av av' stk stk' wpre wsuf wsuf' hwf hi hs.
+  unfold step in hs.
+  destruct stk as (fr, frs).
+  destruct fr as [(xo, rpre, rsuf) v].
+  destruct rsuf.
+  - destruct frs as [| fr_cr frs].
+    + destruct wsuf; tc.
+    + destruct fr_cr as [(xo_cr, rpre_cr, rsuf_cr) v_cr].
+      destruct rsuf_cr as [| [a | x] rsuf_cr]; tc.
+      (* return case *)
+      inv hs.
+      inv hwf.
+      inv hi.
+      rename wpre0 into wpre.
+      exists (wpre ++ wpre'); split; auto.
+      eapply foo; eauto.
+      rewrite app_nil_r; auto.
+  - destruct s as [a | x].
+    + destruct wsuf as [| (a', l) wsuf]; tc.
+      destruct (t_eq_dec a' a); tc; subst.
+      inv hs.
+      exists (wpre ++ [(a, l)]).
+      split.
+      * rewrite <- app_assoc; auto.
+      * eapply foo'; eauto. 
+    + destruct (NtSet.mem x av); tc.
+      dmeq hpred; tc.
+      * inv hs.
+        exists wpre; split; auto.
+        assert (happ : wpre = wpre ++ []) by apply app_nil_r'; rewrite happ.
+        constructor; auto.
+        constructor.
+      * inv hs.
+        exists wpre; split; auto.
+        assert (happ : wpre = wpre ++ []) by apply app_nil_r'.
+        rewrite happ; constructor; auto.
+        constructor.
+Qed.
+    
+
+(*
+(* maybe we need a four-place derivation relation including a remainder? *)
+Lemma foo :
+  forall g bfr bfr' av av' stk stk' ts ts' vsuf,
+    bottom_frame bfr stk
+    -> bottom_frame bfr' stk'
+    -> step g (Pst av stk ts) = StepK (Pst av' stk' ts')
+    -> gamma_derivation g bfr'.(loc).(rsuf) ts' vsuf
+    -> exists w v,
+        bfr.(sem) ++ v = bfr'.(sem) ++ vsuf
+        /\ gamma_derivation g bfr.(loc).(rsuf) (w ++ ts) v.
+Proof.
+  intros g bfr bfr' av av' stk stk' ts ts' vsuf hbf hbf' hs hg.
+  unfold step in hs.
+  destruct stk as (fr, frs).
+  destruct fr as [[xo pre suf] v].
+  destruct suf as [| [a | x] suf_tl].
+  - destruct frs as [| fr_cr frs].
+    + destruct ts; tc.
+    + destruct fr_cr as [[xo_cr pre_cr suf_cr] v_cr].
+      (* we should know that the frame derivation invariant holds in the callee *)
+      assert (hgd : exists w, gamma_derivation g pre w v) by admit.
+      destruct hgd as [w hgd].
+      destruct suf_cr as [| [a | x] suf_tl_cr]; tc.
+      (* we should also know that (x, pre ++ suf) is a grammar production *)
+      assert (hpr : In (x, pre) g) by admit.
+      inv hs.
+      inv hbf.
+      destruct frs.
+      * inv hbf'; inv H1.
+        simpl in *.
+        exists w; exists (Node x v :: vsuf).
+        split.
+        -- rewrite <- app_assoc; auto.
+        -- constructor; auto.
+           econstructor; eauto.
+      * inv hbf'; inv H1.
+        assert (bfr' = bfr) by admit; subst.
+        exists nil; eexists; split; eauto.
+  - destruct ts as [| (a', l) ts_tl]; tc.
+    destruct (t_eq_dec a' a); tc; subst.
+    inv hs.
+    destruct frs.
+    + inv hbf; inv hbf'.
+      simpl in *.
+      exists []; exists (Leaf l :: vsuf); split.
+      * rewrite <- app_assoc; auto.
+      * simpl.
+        admit.
+    + inv hbf; inv hbf'.
+      assert (bfr = bfr') by admit; subst.
+Abort.
+
 Lemma multistep_sound :
   forall (g   : grammar)
          (ts  : list token)
          (av  : NtSet.t)
          (stk : p_stack)
-         a
-         (trs : forest),
-    multistep g (Pst av stk ts) a = Accept trs
-    -> exists trs_suf,
-      trs = (bottomFrame stk).(sem) ++ trs_suf
-      /\ gamma_derivation g (bottomFrame stk).(loc).(rsuf) ts trs_suf.
+         (a   : Acc lex_nat_triple (meas g (Pst av stk ts)))
+         (v   : forest)
+         (fr  : frame),
+    bottom_frame fr stk
+(*    -> frame_derivation_invar g fr *)
+    -> multistep g (Pst av stk ts) a = Accept v
+    -> exists vsuf,
+      v = fr.(sem) ++ vsuf
+      /\ gamma_derivation g fr.(loc).(rsuf) ts vsuf.
 Proof.
-  (* nested induction on lexicographic components of the multistep measure *)
-  intros g ts; induct_list_length ts.
-  intros av stk; induct_stackScore g av stk.
-  (*remember (stackHeight stk) as ht eqn:Hht.
-  generalize dependent stk.
-  induction ht as [ht IHht] using lt_wf_ind.
-  intros stk IHsc Hht; subst. *)
-  intros a trs hm.
-  apply multistep_accept in hm.
+Abort.
+*)
+
+Lemma multistep_sound :
+  forall (g   : grammar)
+         (ts  : list token)
+         (av  : NtSet.t)
+         (stk : p_stack)
+         (a   : Acc lex_nat_triple (meas g (Pst av stk ts)))
+         (v   : forest)
+         (fr  : frame),
+    bottom_frame fr stk
+(*    -> frame_derivation_invar g fr *)
+    -> multistep g (Pst av stk ts) a = Accept v
+    -> exists vsuf,
+      v = fr.(sem) ++ vsuf
+      /\ gamma_derivation g fr.(loc).(rsuf) ts vsuf.
+Proof.
+  intros g ts.
+  induct_list_length ts.
+  intros av stk a v fr hbf hm.
+  apply multistep_accept_cases in hm.
   destruct hm as [hs | he].
-  - clear IHl; clear IHsc.
-    (* prove that if some "partial derivation" invariant holds of the parser state,
-       this goal is provable *)
-    admit.
-  - destruct he as [st' [a' [hs hm]]].
+  - (* the parser state is in a "final configuration" *)
+    apply step_StepAccept_facts in hs.
+    destruct hs as [[xo [rpre [v' [heq]]]] heq']; subst.
+    inv hbf.
+    exists []; split; simpl; [rewrite app_nil_r; auto | constructor].
+  - (* parser is in a non-final configuration *)
+    destruct he as [st' [a' [hs hm]]].
+    destruct st' as [av' stk' ts'].
+    assert (hl : length ts' < length ts) by admit.
+    assert (hex : exists fr', bottom_frame fr' stk') by admit.
+    destruct hex as [fr' hbf'].
+    eapply IHl with (m := length ts')
+                    (ts := ts')
+                    (av := av')
+                    (stk := stk')
+                    (fr  := fr') in hl; eauto.
+    destruct hl as [vsuf [heq hgd]]; subst.
+    clear IHl.
+    eapply foo; eauto.
     (* I think the induction hypotheses will give me this one. I might also
        have to prove that "step" preserves whatever invariant I used in the
        previous goal. *)
-    admit.
 Admitted.
+
 
 Theorem parser_sound :
   forall (g : grammar)
          (ss : list symbol)
          (ts : list token)
-         (trs : forest),
-    parse g ss ts = Accept trs -> gamma_derivation g ss ts trs.
+         (v : forest),
+    parse g ss ts = Accept v
+    -> gamma_derivation g ss ts v.
 Proof.
-  intros g ss ts trs Hp.
-  unfold parse in Hp.
-  apply multistep_sound in Hp.
-  destruct Hp as [trs_suf [Heq Hd]]; subst; simpl in *; auto.
+  intros g ss ts v hp.
+  unfold parse in hp.
+  eapply multistep_sound with (fr := Fr (Loc None [] ss) []) in hp.
+  - destruct hp as [vsuf [heq hgd]]; subst; simpl in *; auto.
+  - constructor; auto.
 Qed.
   
